examples/enumProofs.v
@@ -382,3 +382,4 @@ Inductive goodTree : nat -> tree nat  -> Prop :=
       goodTree m t1 ->
       goodTree (S n) (Node nat k t1 t2).
 
+
